---
layout: post
title:  9跨过黄河求距离_解三角形
date:   2022-11-31
author: 黄靖旻
categories: course zhi-xin shu-xue gao-zhong-shu-xue
---

## 一、三角恒等变换

$$
\begin{aligned}
    \cos (\alpha - \beta) & = \cos \alpha \cos \beta + \sin \alpha \sin \beta \\
    \cos (\alpha + \beta) & = \cos (\alpha + (- \beta)) \\
    & = \cos \alpha \cos (- \beta) + \sin \alpha \sin (- \beta) \\
    & = \cos \alpha \cos \beta - \sin \alpha \sin \beta \\
    \sin (\alpha + \beta) & = \cos \alpha \sin \beta + \sin \alpha \cos \beta \\
    \sin (\alpha - \beta) & = \sin \alpha \cos \beta - \cos \alpha \sin \beta \\
    \tan (\alpha + \beta) & = \frac{\sin (\alpha + \beta)}{\cos (\alpha + \beta)} \\
    & = \frac{\sin \alpha \cos \beta + \sin \beta \cos \alpha}{\cos \alpha \cos \beta - \sin \alpha \sin \beta} \\
    & = \frac{\frac{\sin \alpha}{\cos \alpha} + \frac{\sin \beta}{\cos \beta}}{1 - \frac{\sin \alpha}{\cos \alpha} \frac{\sin \beta}{\cos \beta}} \\
    & = \frac{\tan \alpha + \tan \beta}{1 - \tan \alpha \tan \beta} \\
    \tan (\alpha - \beta) & = \tan (\alpha + (- \beta)) \\
    & = \frac{\tan \alpha - \tan \beta}{1 + \tan \alpha \tan \beta}
\end{aligned}
$$

### 和差化积

$$
\begin{aligned}
    帅 + 帅 & = 帅哥 && \sin \alpha + \sin \beta = 2 \sin \frac{\alpha + \beta}{2} \cos \frac{\alpha - \beta}{2}\\
    帅 - 帅 & = 哥帅 && \sin \alpha - \sin \beta = 2 \cos \frac{\alpha + \beta}{2} \sin \frac{\alpha - \beta}{2} \\
    哥 + 哥 & = 哥哥 && \cos \alpha + \cos \beta = 2 \cos \frac{\alpha + \beta}{2} \cos \frac{\alpha - \beta}{2}\\
    哥 - 哥 & = 负嫂嫂 && \cos \alpha - \cos \beta = - 2 \sin \frac{\alpha + \beta}{2} \sin \frac{\alpha - \beta}{2}\\ 
\end{aligned}
$$

### 二倍角公式

### 半倍角公式

## 二、解三角形——正弦定理

$$\frac{a}{\sin A} = \frac{b}{\sin B} = \frac{c}{\sin C} = 2 R$$

## 三、余弦定理

$$
\begin{aligned}
    a^2 & = b^2 + c^2 - 2 bc \cos A \\
    b^2 & = c^2 + a^2 - 2 ac \cos B \\
    c^2 & = a^2 + b^2 - 2 ab \cos C
\end{aligned}
$$

$$
\begin{aligned}
    \cos A & = \frac{b^2 + c^2 - a^2}{2 bc} \\
    \cos B & = \frac{a^2 + c^2 - b^2}{2 ac} \\
    \cos C & = \frac{a^2 + b^2 - b^2}{2 ab} \\
\end{aligned}
$$

$$
\begin{aligned}
    a & = b \cos C + c \cos B \\
    b & = c \cos A + a \cos C \\
    c & = b \cos A + a \cos B
\end{aligned}
$$